impl/dafny/generic_dw_add.i.dfy
@@ -1,0 +1,69 @@
+include "../../lib/generic_bv_ops.dfy"
+include "../../lib/bv256_ops.dfy"
+
+abstract module generic_dw_add {
+    import opened GBV: generic_bv_ops
+    import opened BVSEQ = GBV.BVSEQ
+    import opened Mul
+    import opened Power
+    import opened DivMod
+    import integers
+
+    // type uint = GBV.BVSEQ.uint
+
+    predicate dw_add_is_safe(
+        x_lh: uint, x_uh: uint,
+        y_lh: uint, y_uh: uint)
+    {
+        ToNatRight([x_lh, x_uh]) + ToNatRight([y_lh, y_uh]) < DW_BASE()
+    }
+
+    lemma dw_add_lemma(
+        x_lh: uint, x_uh: uint,
+        y_lh: uint, y_uh: uint,
+        c1: integers.uint1, c2: integers.uint1,
+        z_lh: uint, z_uh: uint)
+
+        requires dw_add_is_safe(x_lh, x_uh, y_lh, y_uh);
+        requires (z_lh, c1) == GBV.addc(x_lh, y_lh, 0);
+        requires (z_uh, c2) == GBV.addc(x_uh, y_uh, c1);
+        
+        ensures ToNatRight([z_lh, z_uh]) == ToNatRight([x_lh, x_uh]) + ToNatRight([y_lh, y_uh]);
+    {
+        var x_full := ToNatRight([x_lh, x_uh]);
+        var y_full := ToNatRight([y_lh, y_uh]);
+        var z_full := ToNatRight([z_lh, z_uh]);
+
+        assert SeqAdd([x_lh], [y_lh]) == ([z_lh], c1) by {
+            reveal SeqAdd();
+            assert [] + [z_lh] == [z_lh];
+        }
+
+        assert SeqAdd([x_lh, x_uh], [y_lh, y_uh]) == ([z_lh, z_uh], c2) by {
+            reveal SeqAdd();
+            assert [z_lh] + [z_uh] == [z_lh, z_uh];
+        }
+
+        assert ToNatRight([z_lh, z_uh]) + c2 * Pow(BASE(), 2) == x_full + ToNatRight([y_lh, y_uh]) by {
+            LemmaSeqAdd([x_lh, x_uh], [y_lh, y_uh], [z_lh, z_uh], c2);
+        }
+
+        if c2 != 0 {
+            reveal Pow();
+            assert false;
+        }
+    }
+
+    method dw_add(x_lh: uint, x_uh: uint, y_lh: uint, y_uh: uint)
+        requires dw_add_is_safe(x_lh, x_uh, y_lh, y_uh);
+    {
+        var (z_lh, c1) := GBV.addc(x_lh, y_lh, 0);
+        var (z_uh, c2) := GBV.addc(x_uh, y_uh, c1);
+        dw_add_lemma(x_lh, x_uh, y_lh, y_uh, c1, c2, z_lh, z_uh);
+    }
+}
+
+module bv256_dw_add refines generic_dw_add {
+    import opened GBV = bv256_ops
+    import opened BVSEQ = bv256_seq
+}
